WIP termination proof, state type
Introduced a type_synonym to abbreviate the state of the search_step algorithm. This should make it shorter and easier to read.

A rudimentary termination proof has been finished, but it needs polishing that will not happen until a thesis draft is completed.

TangleLearning_Search.thy
@@ -1,6 +1,8 @@
 theory TangleLearning_Search
-imports Main TangleAttractors TangleLearning
+imports Main PredicateTermination TangleAttractors TangleLearning
 begin
+
+type_synonym 'a search_state = "'a set \<times> 'a set set"
 
 context paritygame begin
 
@@ -24,7 +26,7 @@ context
 begin
 
 (** search_step represents a single iteration of the while-loop in the search algorithm. *)
-inductive search_step :: "'v set \<times> 'v set set \<Rightarrow> 'v set \<times> 'v set set \<Rightarrow> bool" where
+inductive search_step :: "'v search_state \<Rightarrow> 'v search_state \<Rightarrow> bool" where
   step:
   "\<lbrakk>R \<noteq> {};
     p = pr_set R; \<alpha> = player_wins_pr p;
@@ -57,19 +59,19 @@ definition search_I ::  "'v set \<times> 'v set set \<Rightarrow> bool" where
   "search_I S \<equiv> finite (snd S) \<and> (\<forall>U \<in> snd S. \<exists>\<alpha>. tangle \<alpha> U) \<and> (fst S={} \<longrightarrow> \<dots>)"
 *)
 
-definition search_I :: "'v set \<times> 'v set set \<Rightarrow> bool" where
+definition search_I :: "'v search_state \<Rightarrow> bool" where
   "search_I \<equiv> \<lambda>(R,Y). finite R \<and> valid_subgame R \<and> finite Y \<and> (\<forall>U \<in> Y. \<exists>\<alpha>. tangle \<alpha> U)"
 
 (** If we end with an empty region, then we have a finite, non-empty Y containing new tangles that
     were not included in T before, as specified by our invariant. *)
 lemma search_I_correct:
   "search_I ({},Y) \<Longrightarrow> finite Y \<and> Y \<noteq> {} \<and> (\<forall>U \<in> Y. \<exists>\<alpha>. tangle \<alpha> U \<and> U \<notin> T)"
-  unfolding search_I_def apply simp sorry
+  unfolding search_I_def apply simp oops
 
 (** If the initial R is finite, then R' is finite after a step. *)
 lemma search_step_R_finite:
   "\<lbrakk>search_step (R,Y) (R',Y'); finite R\<rbrakk> \<Longrightarrow> finite R'"
-  apply (induction rule: search_step_induct) by blast
+  by (induction rule: search_step_induct) blast
 
 (** If the initial R is a valid subgame, then R' is a valid subgame after a step. *)
 lemma search_step_valid_subgame:
@@ -115,38 +117,41 @@ proof (induction rule: search_step_induct)
   from R_valid_game interpret R_game:
     paritygame "Restr E R" "V\<inter>R" "V\<^sub>0\<inter>R" by blast
 
+  let ?G\<sigma> = "induced_subgraph \<sigma>"
+  let ?G\<sigma>_V = "induced_subgraph_V \<sigma>"
+
   from A_def \<open>R \<subseteq> V\<close>
     R_game.target_in_tangle_attractor[OF fin_T attr]
     R_game.tangle_attractor_in_V[OF fin_T attr]
-  have A_in_Z: "A \<subseteq> Z" and Z_in_R: "Z \<subseteq> R" by auto
+  have "A \<subseteq> Z" and "Z \<subseteq> R" and "A \<subseteq> R" by auto
   with R_in_V R_game.player_strat_in_E
     R_game.tangle_attractor_strat[OF fin_T attr] have
     \<sigma>_strat: "strategy_of (V_player \<alpha> \<inter> Z) \<sigma>" and
     \<sigma>_dom: "dom \<sigma> \<subseteq> V_player \<alpha> \<inter> Z" and
     \<sigma>_ran: "ran \<sigma> \<subseteq> Z" and
-    \<sigma>_partially_closed: "(Restr (induced_subgraph \<sigma>) R) `` (Z-A) \<subseteq> Z" and
+    \<sigma>_partially_closed: "(Restr ?G\<sigma> R) `` (Z-A) \<subseteq> Z" and
     \<sigma>_forces_A_or_wins:
-      "\<forall>x\<in>Z. \<forall>xs ys. lasso (Restr (induced_subgraph \<sigma>) R) x xs ys
+      "\<forall>x\<in>Z. \<forall>xs ys. lasso (Restr ?G\<sigma> R) x xs ys
         \<longrightarrow>set (xs @ ys) \<inter> A \<noteq> {} \<or> player_wins_list \<alpha> ys" and
     \<sigma>_path_to_A:
-      "\<forall>x\<in>Z. \<exists>y\<in>A. \<exists>xs. path (Restr (induced_subgraph \<sigma>) R) x xs y"
+      "\<forall>x\<in>Z. \<exists>y\<in>A. \<exists>xs. path (Restr ?G\<sigma> R) x xs y"
     unfolding restr_subgraph_V_player[OF R_valid_game]
       restr_ind_subgraph[OF paritygame.axioms[OF R_valid_game]]
     unfolding strategy_of_player_def strategy_of_def by auto
 
   have all_games_in_Z_won:
-    "\<forall>v\<in>Z. \<forall>xs ys. lasso (Restr (induced_subgraph \<sigma>) Z) v xs ys
+    "\<forall>v\<in>Z. \<forall>xs ys. lasso (Restr ?G\<sigma> Z) v xs ys
       \<longrightarrow> player_wins_list \<alpha> ys"
   proof -
-    from R_in_V step(2,3) have "player_winningP \<alpha> (pr_set (V \<inter> R))"
+    from \<open>R\<subseteq>V\<close> step(2,3) have "player_winningP \<alpha> (pr_set (V \<inter> R))"
       by (cases \<alpha>; simp add: player_wins_pr_def Int_absorb1 split: if_splits)
-    moreover from R_in_V step(2,4) have "A = {v \<in> V \<inter> R. pr v = pr_set (V \<inter> R)}"
+    moreover from \<open>R\<subseteq>V\<close> step(2,4) have "A = {v \<in> V \<inter> R. pr v = pr_set (V \<inter> R)}"
       by (simp add: Int_absorb1)
     ultimately show ?thesis
       using R_game.van_dijk_2[OF fin_T _ _ attr]
       unfolding restr_subgraph_V_player[OF R_valid_game]
         restr_ind_subgraph[OF paritygame.axioms[OF R_valid_game]]
-        Restr_subset[OF Z_in_R] by simp
+        Restr_subset[OF \<open>Z\<subseteq>R\<close>] by simp
   qed
 
   show ?case
@@ -158,35 +163,35 @@ proof (induction rule: search_step_induct)
       case old with tangles_Y show ?thesis by blast
     next
       case new
-      from new have U_in_Z: "U \<subseteq> Z" by blast
-      with R_in_V Z_in_R have U_in_V: "U \<subseteq> V" by blast
+      from new have "U \<subseteq> Z" by blast
+      with \<open>Z\<subseteq>R\<close> have "U \<subseteq> R" by blast
+      with \<open>R\<subseteq>V\<close> have "U \<subseteq> V" by blast
       from finite_subset[OF this fin_V] have fin_U: "finite U" .
-      from new have U_notempty: "U \<noteq> {}"
+      from new have "U \<noteq> {}"
         using finite_graph_V.nt_bottom_SCC_notempty by force
 
-      let ?\<sigma>_graph = "induced_subgraph \<sigma>"
-      let ?\<sigma>_graph_V = "induced_subgraph_V \<sigma>"
-      interpret fin_graph_\<sigma>: finite_graph_V ?\<sigma>_graph ?\<sigma>_graph_V by simp
+      interpret fin_graph_\<sigma>: finite_graph_V ?G\<sigma> ?G\<sigma>_V by simp
 
-      from new U_in_V have \<sigma>_connected: "strongly_connected (Restr ?\<sigma>_graph U) U"
+      from new \<open>U\<subseteq>V\<close> have \<sigma>_connected: "strongly_connected (Restr ?G\<sigma> U) U"
         using fin_graph_\<sigma>.nt_bottom_SCC_strongly_connected fin_graph_\<sigma>.nt_bottom_SCC_in_V
         by (simp add: Int_absorb1)
-      from new have \<sigma>_U_succ_in_U: "\<forall>v\<in>U. \<exists>v'\<in>U. (v,v') \<in> ?\<sigma>_graph"
+      from new have \<sigma>_U_succ_in_U: "\<forall>v\<in>U. \<exists>v'\<in>U. (v,v') \<in> ?G\<sigma>"
         using fin_graph_\<sigma>.nt_bottom_SCC_succ_in_SCC by blast
 
       define \<sigma>' where "\<sigma>' = \<sigma> |` U"
-      let ?\<sigma>'_graph = "induced_subgraph \<sigma>'"
-      let ?\<sigma>'_graph_V = "induced_subgraph_V \<sigma>'"
+      let ?G\<sigma>' = "induced_subgraph \<sigma>'"
+      let ?G\<sigma>'_V = "induced_subgraph_V \<sigma>'"
       have \<sigma>'_le_\<sigma>: "\<sigma>' \<subseteq>\<^sub>m \<sigma>" by (auto simp: \<sigma>'_def map_le_def)
 
-      from restricted_strat_subgraph_same_in_region[OF \<sigma>'_def] have graphs_equal_in_U:
-        "Restr ?\<sigma>_graph U = Restr ?\<sigma>'_graph U" .
+      from restricted_strat_subgraph_same_in_region[OF \<sigma>'_def]
+      have graphs_equal_in_U:
+        "Restr ?G\<sigma> U = Restr ?G\<sigma>' U" .
       from restricted_strat_subgraph_V_same_in_region[OF \<sigma>'_def] new
-      have graph_V_equal_in_U: "?\<sigma>_graph_V \<inter> U = ?\<sigma>'_graph_V \<inter> U"
+      have graph_V_equal_in_U: "?G\<sigma>'_V \<inter> U = ?G\<sigma>_V \<inter> U"
         using fin_graph_\<sigma>.nt_bottom_SCC_in_V by blast
 
       from \<sigma>_U_succ_in_U graphs_equal_in_U have \<sigma>'_U_succ_in_U:
-        "\<forall>v\<in>U. \<exists>v'\<in>U. (v, v') \<in> induced_subgraph \<sigma>'" by blast
+        "\<forall>v\<in>U. \<exists>v'\<in>U. (v, v') \<in> ?G\<sigma>'" by blast
 
       from \<sigma>_strat have \<sigma>'_strat: "strategy_of (V_player \<alpha>) \<sigma>'"
         using strat_le_E_of_strat[OF \<sigma>'_le_\<sigma>]
@@ -198,17 +203,17 @@ proof (induction rule: search_step_induct)
       next
         {
           fix x assume assm: "x \<in> V_player \<alpha> \<inter> A \<inter> U"
-          with U_in_Z Z_in_R \<sigma>'_U_succ_in_U
+          with \<open>U\<subseteq>R\<close> \<sigma>'_U_succ_in_U
           have "Restr E R `` {x} \<inter> U \<noteq> {}"
             using ind_subgraph by fast
-          with assm U_in_Z have "x \<in> dom \<sigma>'"
+          with assm \<open>U\<subseteq>Z\<close> have "x \<in> dom \<sigma>'"
             using R_game.tangle_attractor_strat_in_dom_A[OF fin_T attr]
             unfolding restr_subgraph_V_player[OF R_valid_game] \<sigma>'_def by auto
         }
         moreover
         {
           fix x assume "x \<in> V_player \<alpha> \<inter> (U-A)"
-          with Z_in_R U_in_Z have "x \<in> dom \<sigma>'"
+          with \<open>U\<subseteq>Z\<close> \<open>Z\<subseteq>R\<close> have "x \<in> dom \<sigma>'"
             using R_game.tangle_attractor_strat_in_dom_not_A[OF fin_T attr, of x]
             unfolding restr_subgraph_V_player[OF R_valid_game] \<sigma>'_def by fastforce
         }
@@ -221,17 +226,17 @@ proof (induction rule: search_step_induct)
 
       from \<sigma>_connected have \<sigma>'_connected:
         "strongly_connected (tangle_subgraph \<alpha> U \<sigma>') U"
-        unfolding tangle_subgraph_is_restricted_ind_subgraph[OF U_in_V \<sigma>'_dom \<sigma>'_ran]
+        unfolding tangle_subgraph_is_restricted_ind_subgraph[OF \<open>U\<subseteq>V\<close> \<sigma>'_dom \<sigma>'_ran]
         by (simp add: graphs_equal_in_U)
 
-      from U_in_Z have tangle_subgraph_subset:
-        "tangle_subgraph \<alpha> U \<sigma>' \<subseteq> Restr (induced_subgraph \<sigma>) Z"
-        unfolding tangle_subgraph_is_restricted_ind_subgraph[OF U_in_V \<sigma>'_dom \<sigma>'_ran]
+      from \<open>U\<subseteq>Z\<close> have tangle_subgraph_subset:
+        "tangle_subgraph \<alpha> U \<sigma>' \<subseteq> Restr ?G\<sigma> Z"
+        unfolding tangle_subgraph_is_restricted_ind_subgraph[OF \<open>U\<subseteq>V\<close> \<sigma>'_dom \<sigma>'_ran]
         unfolding \<sigma>'_dom
         unfolding restricted_strat_and_dom_subgraph_same_in_region[OF \<sigma>'_def] by blast
       have \<sigma>'_all_cycles_in_U_won:
         "\<forall>v\<in>U. \<forall>xs. cycle (tangle_subgraph \<alpha> U \<sigma>') v xs \<longrightarrow> player_wins_list \<alpha> xs"
-        using subgraph_cycles_won_if_plays_won[OF tangle_subgraph_subset U_in_Z all_games_in_Z_won] .
+        using subgraph_cycles_won_if_plays_won[OF tangle_subgraph_subset \<open>U\<subseteq>Z\<close> all_games_in_Z_won] .
 
       have \<sigma>'_tangle_strat: "tangle_strat \<alpha> U \<sigma>'"
         unfolding tangle_strat_iff Let_def
@@ -254,21 +259,21 @@ proof (induction rule: search_step_induct)
               at least one node in A.
 
               The last step in the former reasoning needs some more work. *)
-          have "\<forall>x\<in>U. \<exists>y\<in>A. \<exists>xs. path (Restr (induced_subgraph \<sigma>') U) x xs y"
+          have "\<forall>x\<in>U. \<exists>y\<in>A. \<exists>xs. path (Restr ?G\<sigma>' U) x xs y"
           proof (rule ballI)
             fix x assume "x \<in> U"
-            show "\<exists>y\<in>A. \<exists>xs. path (Restr (induced_subgraph \<sigma>') U) x xs y" sorry
+            show "\<exists>y\<in>A. \<exists>xs. path (Restr ?G\<sigma>' U) x xs y" sorry
           qed
           show ?thesis sorry
         qed
         hence "pr_set U = pr_set R"
           unfolding step
-          using pr_set_exists[OF fin_U U_notempty]
+          using pr_set_exists[OF fin_U \<open>U\<noteq>{}\<close>]
           using pr_le_pr_set[OF fin_U]
           using R_game.pr_le_pr_set_V
-          apply (safe; clarsimp simp: Int_absorb1[OF R_in_V])
+          apply (safe; clarsimp simp: Int_absorb1[OF \<open>R\<subseteq>V\<close>])
           using le_antisym[of "pr v" "pr_set U" for v]
-          using U_in_Z Z_in_R subset_eq
+          using \<open>U\<subseteq>R\<close> subset_eq
           by metis
         thus ?thesis
           unfolding step player_wins_pr_def by simp
@@ -277,8 +282,8 @@ proof (induction rule: search_step_induct)
       show ?thesis
         unfolding tangle_iff
         apply (rule exI[where x=\<alpha>]; intro conjI)
-        subgoal using U_notempty .
-        subgoal using U_in_V .
+        subgoal using \<open>U\<noteq>{}\<close> .
+        subgoal using \<open>U\<subseteq>V\<close> .
         subgoal using winning_pr_U .
         subgoal using \<sigma>'_tangle_strat by blast
         done
@@ -325,7 +330,7 @@ lemma search_preserves_I:
     new tangles that were not included in T before. *)
 theorem valid_subgame_search_correct:
   "\<lbrakk>valid_subgame R; search R Y\<rbrakk> \<Longrightarrow> finite Y \<and> Y \<noteq> {} \<and> (\<forall>U \<in> Y. \<exists>\<alpha>. tangle \<alpha> U \<and> U \<notin> T)"
-  using search_I_correct[OF search_preserves_I[OF _ I_base_valid_subgame]] by simp
+  using search_I_correct[OF search_preserves_I[OF _ I_base_valid_subgame]] oops
 
 
 section \<open>Termination\<close>
@@ -334,15 +339,13 @@ lemma search_step_R_decreasing:
   "\<lbrakk>search_step (R,Y) (R',Y'); valid_subgame R\<rbrakk> \<Longrightarrow> R' \<subset> R"
   apply (induction rule: search_step_induct)
   subgoal for R
-  using pr_set_exists[OF finite_subset[OF _ fin_V, of R]]
-        paritygame.target_in_tangle_attractor[OF _ fin_T]
-  by blast
+    using pr_set_exists[OF finite_subset[OF _ fin_V, of R]]
+    using paritygame.target_in_tangle_attractor[OF _ fin_T]
+    by blast
   done
 
-term search_step
-find_theorems search_I search_step
-
-lemma search_step_wfP_I: "wfP (\<lambda>s' s. search_step s s' \<and> search_I s)"
+lemma search_step_wfP_I:
+  "wfP (\<lambda>s' s. search_step s s' \<and> search_I s)"
   unfolding wfP_def
   apply (rule wf_subset[of "inv_image (finite_psubset) (\<lambda>(R,Y). R)"]; clarsimp)
   subgoal for R' Y' R Y
@@ -376,31 +379,10 @@ proof (rule ccontr)
   with final show False by blast
 qed
 
-inductive trm for R where
-  "(\<forall>s'. R s s' \<longrightarrow> trm R s') \<Longrightarrow> trm R s"
-
-lemma "\<nexists>s'. R s s' \<Longrightarrow> trm R s"
-  by (simp add: trm.intros)
-
-lemma trm_has_final_state: "trm R s \<Longrightarrow> \<exists>s'. R\<^sup>*\<^sup>* s s' \<and> \<not>Domainp R s'"
-  apply (induction rule: trm.induct)
-  by (metis Domainp.cases converse_rtranclp_into_rtranclp rtranclp.rtrancl_refl)
-
-
-(** A wellfounded relation terminates. *)
-lemma wf_rel_terminates_I:
-  assumes "I s"
-  assumes "\<And>s s'. I s \<Longrightarrow> R s s' \<Longrightarrow> I s'"
-  assumes "wfP (\<lambda>s' s. R s s' \<and> I s)"
-  shows "trm R s"
-  using assms(3,1) apply induction
-  apply (blast intro: trm.intros assms(2))
-  done
-
 lemma search_step_terminates:
   assumes "valid_subgame R"
   shows "trm search_step (R,{})"
-  apply (rule wf_rel_terminates_I[where I=search_I])
+  apply (rule wfP_I_terminates[where I=search_I])
   using I_base_valid_subgame[OF assms(1)]
   using search_step_preserves_I
   using search_step_wfP_I
@@ -409,107 +391,11 @@ lemma search_step_terminates:
 lemma search_step_exists:
   assumes "valid_subgame R"
   shows "\<exists>Y. search R Y"
-  using trm_has_final_state[OF search_step_terminates[OF assms]]
+  using trm_final_state[OF search_step_terminates[OF assms]]
   using I_base_valid_subgame[OF assms]
   using search_step_final_empty_R[OF search_step_rtranclp_preserves_I]
   unfolding search_def by fast
-
-(*
-(** Because R is finite and decreases with every step, search_step is a well-founded relation. *)
-lemma search_step_wellfounded: "wfP (search_step\<inverse>\<inverse>)"
-  unfolding wfP_def
-  apply (rule wf_subset[of "inv_image (finite_psubset) (\<lambda>(R,Y). R)"]; clarsimp)
-  subgoal for R' Y' R Y
-
-    find_theorems name: Tangle name: mono
-
-    using search_step_mono[of "(R,Y)" "(R',Y')"] search_step_R_finite[of "(R,Y)"]
-    by simp
-  done
-*)
-(*
-(** If R is a valid non-empty subgame, then search_step can always be applied.
-    The specifics of Y are not relevant, as it has no preconditions in the step. *)
-lemma search_step_continues_on_valid_R:
-  "\<lbrakk>R \<noteq> {}; R \<subseteq> V; paritygame (Restr E R) (V\<inter>R) (V\<^sub>0\<inter>R)\<rbrakk> \<Longrightarrow> Domainp search_step (R,Y)"
-proof -
-  assume R_notempty: "R\<noteq>{}" and
-         R_in_V: "R \<subseteq> V" and
-         R_valid_subgame: "paritygame (Restr E R) (V\<inter>R) (V\<^sub>0\<inter>R)"
-  (** All we have to do is define the local variables with their conditions in the step. *)
-  moreover define p where "p = pr_set R"
-  moreover define \<alpha> where "\<alpha> = player_wins_pr p"
-  moreover define A where "A = {v. v\<in>R \<and> pr v = p}"
-  moreover define T\<^sub>\<alpha> where "T\<^sub>\<alpha> = {t. t \<in> T \<and> paritygame.tangle (Restr E R) (V\<inter>R) (V\<^sub>0\<inter>R) pr \<alpha> t}"
-  moreover from T\<^sub>\<alpha>_def have
-    tangles_T\<^sub>\<alpha>: "\<forall>t\<in>T\<^sub>\<alpha>. paritygame.tangle (Restr E R) (V\<inter>R) (V\<^sub>0\<inter>R) pr \<alpha> t" and
-    fin_T\<^sub>\<alpha>: "finite T\<^sub>\<alpha>"
-    using finite_subset[OF _ fin_T] by auto
-  moreover obtain Z \<sigma> where
-    "paritygame.tangle_attractor (Restr E R) (V\<inter>R) (V\<^sub>0\<inter>R) pr \<alpha> T\<^sub>\<alpha> A Z \<sigma>"
-    using paritygame.tangle_attractor_exists[OF R_valid_subgame tangles_T\<^sub>\<alpha> fin_T\<^sub>\<alpha>] by blast
-  moreover define V\<^sub>\<alpha> where "V\<^sub>\<alpha> = V_player \<alpha>"
-  moreover define V\<^sub>\<beta> where "V\<^sub>\<beta> = V_opponent \<alpha>"
-  moreover define Ov where
-    "Ov = {v. v \<in> V\<^sub>\<alpha>\<inter>A \<and> E `` {v} \<inter> Z \<noteq> {}} \<union> {v. v \<in> V\<^sub>\<beta>\<inter>A \<and> (E `` {v}) \<inter> R \<subseteq> Z}"
-  moreover define Y' where "Y' = (if Ov \<noteq> {} then
-      Y \<union> {S. S \<subseteq> Z \<and> finite_graph_V_Succ.nt_bottom_SCC (induced_subgraph V\<^sub>\<alpha> \<sigma>) (induced_subgraph_V V\<^sub>\<alpha> \<sigma>) S}
-   else
-      Y)"
-  moreover define R' where "R' = R-Z"
-  (** Now, we can put them in their place in the step, and our thesis follows automatically. *)
-  ultimately have "search_step (R,Y) (R',Y')"
-    using search_step.step by blast
-  thus ?thesis by blast
-qed
-
-(** If we start from a valid, non-empty subgame, through applying search_step, we will always reach
-    a final state with a corresponding Y. *)
-lemma search_step_terminates_with_Y:
-  "\<lbrakk>fst S \<noteq> {}; fst S \<subseteq> V; paritygame (Restr E (fst S)) (V\<inter>fst S) (V\<^sub>0\<inter>fst S)\<rbrakk>
-  \<Longrightarrow> \<exists>Y. search_step\<^sup>*\<^sup>* S ({},Y)"
-  using search_step_wellfounded
-  unfolding wfP_def
-proof (induction S rule: wf_induct_rule)
-  case (less x)
-  (** Because R in x is a valid non-empty subgame, we know there is a state y that succeeds
-      it in search_step. *)
-  from search_step_continues_on_valid_R[OF less.prems, of "snd x"]
-  have "Domainp search_step x" by simp
-  then obtain y where step_x_y: "search_step x y" by blast
-  (** Now we consider whether R' in the successor y is empty or not. *)
-  consider (empty_R') "fst y = {}" | (nonempty_R') "fst y \<noteq> {}" by blast
-  thus ?case proof cases
-    (** If R' in y is already empty, we clearly have a step from x to an endpoint. *)
-    case empty_R'
-    with step_x_y have "search_step x ({}, snd y)"
-      using surjective_pairing[of y] by auto
-    thus ?thesis by blast
-  next
-    (** If R' is not empty, then we know it is a valid subgame in V by the properties of the
-        step. *)
-    case nonempty_R'
-    moreover from search_step_R_in_V[OF step_x_y] have "fst y \<subseteq> V" ..
-    moreover from step_result_R_is_paritygame[OF step_x_y]
-    have "paritygame (Restr E (fst y)) (V \<inter> fst y) (V\<^sub>0 \<inter> fst y)" .
-    moreover note step_x_y
-    (** By the induction hypothesis, we then know that from y, we can reach a state with an empty
-        R and a valid Y.*)
-    ultimately obtain Y where "search_step\<^sup>*\<^sup>* y ({}, Y)"
-      using less.IH by blast
-    (** We also know you can reach y from x. By the transitivity of the reflexive transitive
-        closure, we can now say that we can reach the state with an empty R from x, via y. *)
-    moreover from step_x_y have "search_step\<^sup>*\<^sup>* x y" by simp
-    ultimately show ?thesis using rtranclp_trans by fast
-  qed
-qed
-
-(** When an empty R is reached, there exist no further steps in the algorithm. *)
-lemma search_terminates_on_empty_R: "\<not>Domainp search_step ({},Y)"
-  using search_step_R_anti_mono[of "({},Y)"]
-  by auto
-*)
 end (** End of context with fixed T. *)
-end (** End of context paritygame *)
+end (** End of context paritygame. *)
 
 end
